src/program_proof/mpaxos/marshal_proof.v
@@ -36,7 +36,30 @@ Lemma wp_Encode (args_ptr:loc) (args:C) :
         ⌜has_encoding enc args⌝ ∗
         own_slice enc_sl byteT 1 enc
   }}}.
-Admitted.
+Proof.
+  iIntros (?) "H HΦ".
+  iNamed "H".
+  wp_lam.
+  wp_pures.
+  wp_loadField. wp_apply (wp_slice_len).
+  iMod (readonly_load with "Hargs_state_sl") as (?) "Hstate_sl".
+  iDestruct (own_slice_small_sz with "[$]") as %Hsz.
+  wp_pures.
+  wp_apply wp_NewSliceWithCap.
+  { apply encoding.unsigned_64_nonneg. }
+  iIntros (?) "Hsl".
+  wp_apply (wp_ref_to).
+  { done. }
+  iIntros (?) "Hptr".
+  wp_pures. wp_loadField. wp_load.
+  wp_apply (wp_WriteInt with "[$]").
+  iIntros (?) "Hsl". wp_store. wp_loadField.
+  wp_load. wp_apply (wp_WriteInt with "[$]").
+  iIntros (?) "Hsl". wp_store. wp_loadField.
+  wp_load. wp_apply (wp_WriteBytes with "[$Hsl $Hstate_sl]").
+  iIntros (?) "[Hsl _]". wp_store.
+  wp_load. iApply "HΦ". iFrame. iPureIntro. done.
+Qed.
 
 Lemma wp_Decode enc enc_sl (args:C) :
   {{{
@@ -47,7 +70,25 @@ Lemma wp_Decode enc enc_sl (args:C) :
   {{{
         args_ptr, RET #args_ptr; own args_ptr args
   }}}.
-Admitted.
+Proof.
+  iIntros (?) "[%Henc Hsl] HΦ".
+  wp_lam. wp_apply wp_ref_to; first done.
+  iIntros (?) "Hptr". wp_pures.
+  wp_apply wp_allocStruct; first by val_ty.
+  iIntros (?) "Hs". wp_pures. wp_load.
+  iDestruct (struct_fields_split with "Hs") as "HH".
+  iNamed "HH". rewrite Henc.
+  wp_apply (wp_ReadInt with "[$]").
+  iIntros (?) "?". wp_pures. wp_storeField.
+  wp_store. wp_load. wp_apply (wp_ReadInt with "[$]").
+  iIntros (?) "Hstate_sl". wp_pures. wp_storeField. wp_store.
+  wp_load. wp_storeField.
+  iMod (readonly_alloc_1 with "Hstate_sl") as "#Hstate_sl".
+  iMod (readonly_alloc_1 with "state") as "#?".
+  iMod (readonly_alloc_1 with "epoch") as "#?".
+  iMod (readonly_alloc_1 with "nextIndex") as "#?".
+  iApply "HΦ". iModIntro. repeat iExists _; iFrame "∗#".
+Qed.
 
 End applyAsFollowerArgs.
 End applyAsFollowerArgs.
@@ -80,7 +121,16 @@ Lemma wp_Encode (reply_ptr:loc) (reply:C) q :
         ⌜has_encoding enc reply⌝ ∗
         own_slice enc_sl byteT 1 enc
   }}}.
-Admitted.
+Proof.
+  iIntros (?) "H HΦ".
+  wp_lam. wp_apply (wp_NewSliceWithCap).
+  { apply encoding.unsigned_64_nonneg. }
+  iIntros (?) "Hsl". wp_apply (wp_ref_to); first by val_ty.
+  iIntros (?) "Hptr". wp_pures. wp_loadField. wp_load.
+  wp_apply (wp_WriteInt with "[$]"). iIntros (?) "Hsl".
+  wp_store. wp_load.
+  iApply "HΦ". iFrame. done.
+Qed.
 
 Lemma wp_Decode enc enc_sl (reply:C) :
   {{{
@@ -91,7 +141,16 @@ Lemma wp_Decode enc enc_sl (reply:C) :
   {{{
         reply_ptr, RET #reply_ptr; own reply_ptr reply 1
   }}}.
-Admitted.
+Proof.
+  iIntros (?) "[%Henc Hsl] HΦ".
+  wp_lam. wp_apply wp_allocStruct; first by val_ty.
+  iIntros (?) "Hs". wp_pures.
+  iDestruct (struct_fields_split with "Hs") as "HH".
+  iNamed "HH". rewrite Henc.
+  wp_apply (wp_ReadInt with "[$]").
+  iIntros (?) "?". wp_pures. wp_storeField.
+  iApply "HΦ". iModIntro. repeat iExists _; iFrame "∗#".
+Qed.
 
 End applyAsFollowerReply.
 End applyAsFollowerReply.
@@ -128,7 +187,25 @@ Lemma wp_Encode (args_ptr:loc) (args:C) q :
         ⌜has_encoding enc args⌝ ∗
         own_slice enc_sl byteT 1 enc
   }}}.
-Admitted.
+Proof.
+  iIntros (?) "H HΦ".
+  iNamed "H".
+  wp_lam. wp_pures. wp_loadField. wp_apply (wp_slice_len).
+  iDestruct (own_slice_small_sz with "[$]") as %Hsz.
+  wp_pures.
+  wp_apply wp_NewSliceWithCap.
+  { apply encoding.unsigned_64_nonneg. }
+  iIntros (?) "Hsl".
+  wp_apply (wp_ref_to).
+  { done. }
+  iIntros (?) "Hptr".
+  wp_pures. wp_loadField. wp_load.
+  wp_apply (wp_WriteInt with "[$]").
+  iIntros (?) "Hsl". wp_store. wp_loadField.
+  wp_load. wp_apply (wp_WriteBytes with "[$]").
+  iIntros (?) "[Hsl _]". wp_store.
+  wp_load. iApply "HΦ". iFrame. iPureIntro. done.
+Qed.
 
 Lemma wp_Decode enc enc_sl (args:C) :
   {{{
@@ -139,7 +216,22 @@ Lemma wp_Decode enc enc_sl (args:C) :
   {{{
         args_ptr, RET #args_ptr; own args_ptr args 1
   }}}.
-Admitted.
+Proof.
+  iIntros (?) "[%Henc Hsl] HΦ".
+  wp_lam. wp_apply wp_ref_to; first done.
+  iIntros (?) "Hptr". wp_pures.
+  wp_apply wp_allocStruct; first by val_ty.
+  iIntros (?) "Hs". wp_pures.
+  wp_apply wp_ref_of_zero; first done.
+  iIntros (?) "Herr". wp_pures. wp_load.
+  iDestruct (struct_fields_split with "Hs") as "HH".
+  iNamed "HH". rewrite Henc.
+  wp_apply (wp_ReadInt with "[$]").
+  iIntros (?) "?". wp_pures. wp_store.
+  wp_store. wp_load. wp_storeField.
+  wp_load. wp_storeField.
+  iApply "HΦ". iModIntro. repeat iExists _; iFrame "∗#".
+Qed.
 
 End applyReply.
 End applyReply.
@@ -172,7 +264,16 @@ Lemma wp_Encode (args_ptr:loc) (args:C) q :
         ⌜has_encoding enc args⌝ ∗
         own_slice enc_sl byteT 1 enc
   }}}.
-Admitted.
+Proof.
+  iIntros (?) "H HΦ".
+  wp_lam. wp_apply (wp_NewSliceWithCap).
+  { apply encoding.unsigned_64_nonneg. }
+  iIntros (?) "Hsl". wp_apply (wp_ref_to); first by val_ty.
+  iIntros (?) "Hptr". wp_pures. wp_loadField. wp_load.
+  wp_apply (wp_WriteInt with "[$]"). iIntros (?) "Hsl".
+  wp_store. wp_load.
+  iApply "HΦ". iFrame. done.
+Qed.
 
 Lemma wp_Decode enc enc_sl (args:C) :
   {{{
@@ -183,7 +284,16 @@ Lemma wp_Decode enc enc_sl (args:C) :
   {{{
         args_ptr, RET #args_ptr; own args_ptr args 1
   }}}.
-Admitted.
+Proof.
+  iIntros (?) "[%Henc Hsl] HΦ".
+  wp_lam. wp_apply wp_allocStruct; first by val_ty.
+  iIntros (?) "Hs". wp_pures.
+  iDestruct (struct_fields_split with "Hs") as "HH".
+  iNamed "HH". rewrite Henc.
+  wp_apply (wp_ReadInt with "[$]").
+  iIntros (?) "?". wp_pures. wp_storeField. wp_pures.
+  iApply "HΦ". iModIntro. repeat iExists _; iFrame "∗#".
+Qed.
 
 End enterNewEpochArgs.
 End enterNewEpochArgs.
@@ -224,7 +334,32 @@ Lemma wp_Encode (args_ptr:loc) (args:C) q :
         ⌜has_encoding enc args⌝ ∗
         own_slice enc_sl byteT 1 enc
   }}}.
-Admitted.
+Proof.
+  iIntros (?) "H HΦ".
+  iNamed "H".
+  wp_lam.
+  wp_pures.
+  wp_loadField. wp_apply (wp_slice_len).
+  iMod (readonly_load with "Hreply_ret_sl") as (?) "Hstate_sl".
+  iDestruct (own_slice_small_sz with "[$]") as %Hsz.
+  wp_pures.
+  wp_apply wp_NewSliceWithCap.
+  { apply encoding.unsigned_64_nonneg. }
+  iIntros (?) "Hsl".
+  wp_apply (wp_ref_to).
+  { done. }
+  iIntros (?) "Hptr".
+  wp_pures. wp_loadField. wp_load.
+  wp_apply (wp_WriteInt with "[$]").
+  iIntros (?) "Hsl". wp_store. wp_loadField.
+  wp_load. wp_apply (wp_WriteInt with "[$]").
+  iIntros (?) "Hsl". wp_store. wp_loadField.
+  wp_load. wp_apply (wp_WriteInt with "[$]").
+  iIntros (?) "Hsl". wp_store. wp_loadField.
+  wp_load. wp_apply (wp_WriteBytes with "[$Hsl $Hstate_sl]").
+  iIntros (?) "[Hsl _]". wp_store.
+  wp_load. iApply "HΦ". iFrame. iPureIntro. done.
+Qed.
 
 Lemma wp_Decode enc enc_sl (args:C) :
   {{{
@@ -235,34 +370,142 @@ Lemma wp_Decode enc enc_sl (args:C) :
   {{{
         args_ptr, RET #args_ptr; own args_ptr args 1
   }}}.
-Admitted.
-
-Global Instance enterNewEpochReply_fractional args_ptr args :
-  fractional.Fractional (λ q : Qp, own args_ptr args q).
 Proof.
-  rewrite /own.
-  unfold fractional.Fractional.
-  iIntros.
-  iSplit.
-  {
-    iIntros "H". iDestruct "H" as (?) "H".
-    admit.
-  }
-  admit.
-Admitted.
-
-Global Instance enterNewEpochReply_as_fractional args_ptr args q :
-  fractional.AsFractional (own args_ptr args q) (λ q : Qp, own args_ptr args q) q.
-Proof.
-  split; auto; apply _.
+  iIntros (?) "[%Henc Hsl] HΦ".
+  wp_lam. wp_apply wp_allocStruct; first by val_ty.
+  iIntros (?) "Hs". wp_pures. wp_apply wp_ref_to; first done.
+  iIntros (?) "Hptr". wp_pures. wp_apply wp_ref_of_zero; first done.
+  iIntros (?) "Herr". wp_pures. wp_load.
+  iDestruct (struct_fields_split with "Hs") as "HH".
+  iNamed "HH". rewrite Henc.
+  wp_apply (wp_ReadInt with "[$]").
+  iIntros (?) "?". wp_pures. wp_store. wp_store.
+  wp_load. wp_storeField.
+  wp_load. wp_apply (wp_ReadInt with "[$]").
+  iIntros (?) "Hstate_sl". wp_pures. wp_storeField. wp_store.
+  wp_load. wp_apply (wp_ReadInt with "[$]").
+  iIntros (?) "Hstate_sl". wp_pures. wp_storeField. wp_store.
+  wp_load. wp_storeField.
+  iMod (readonly_alloc_1 with "Hstate_sl") as "#Hstate_sl".
+  iApply "HΦ". iModIntro. repeat iExists _; iFrame "∗#".
 Qed.
 
-(* FIXME: *)
-Global Instance enterNewEpochReply_as_mapsto args_ptr args :
-  AsMapsTo (own args_ptr args 1) (λ q : Qp, own args_ptr args q).
-Proof.
-(*   constructor; auto; intros; apply _. *)
-Admitted.
+End enterNewEpochReply.
+End enterNewEpochReply.
 
-End enterNewEpochReply.
-End enterNewEpochReply.
+
+Module paxosState.
+Section paxosState.
+Record t :=
+  mk {
+      epoch : u64;
+      acceptedEpoch : u64 ;
+      nextIndex : u64 ;
+      state : list u8 ;
+      isLeader : bool ;
+    }.
+
+Definition encode (st:t) : list u8 :=
+  u64_le st.(epoch) ++
+  u64_le st.(acceptedEpoch) ++
+  u64_le st.(nextIndex) ++
+  u64_le (if st.(isLeader) then U64 1 else U64 0) ++
+  st.(state)
+.
+
+#[global]
+Instance encode_inj : Inj (=) (=) encode.
+Proof.
+  intros ???. destruct x, y.
+  apply app_inj_1 in H as [? H]; last done.
+  apply app_inj_1 in H as [? H]; last done.
+  apply app_inj_1 in H as [? H]; last done.
+  apply app_inj_1 in H as [? H]; last done.
+  simpl in *.
+  apply (f_equal le_to_u64) in H0, H1, H2.
+  repeat rewrite u64_le_to_word in H0, H1, H2.
+  subst. f_equal. destruct isLeader0, isLeader1; done.
+Qed.
+
+Context `{!heapGS Σ}.
+Definition own_vol (s:loc) (st: paxosState.t) : iProp Σ :=
+  ∃ state_sl,
+  "Hepoch" ∷ s ↦[paxosState :: "epoch"] #st.(epoch) ∗
+  "HaccEpoch" ∷ s ↦[paxosState :: "acceptedEpoch"] #st.(acceptedEpoch) ∗
+  "HnextIndex" ∷ s ↦[paxosState :: "nextIndex"] #st.(nextIndex) ∗
+  "Hstate" ∷ s ↦[paxosState :: "state"] (slice_val state_sl) ∗
+  "#Hstate_sl" ∷ readonly (own_slice_small state_sl byteT 1 st.(state)) ∗
+  "HisLeader" ∷ s ↦[paxosState :: "isLeader"] #st.(isLeader)
+.
+Lemma wp_boolToU64 (b:bool) :
+  {{{ True }}}
+    boolToU64 #b
+  {{{ RET #((if b then U64 1 else U64 0) : u64); True }}}.
+Proof.
+  iIntros (?) "_ HΦ".
+  wp_lam. wp_if_destruct; by iApply "HΦ".
+Qed.
+
+Lemma wp_encode s st :
+  {{{
+        own_vol s st
+  }}}
+    encodePaxosState #s
+  {{{
+        sl, RET (slice_val sl);
+        own_vol s st ∗
+        own_slice sl byteT 1 (encode st)
+  }}}
+.
+Proof.
+  iIntros (?) "H HΦ".
+  iNamed "H".
+  wp_lam. wp_apply (wp_NewSlice).
+  iIntros (?) "Hsl". wp_apply (wp_ref_to); first done.
+  iIntros (?) "Hptr". wp_pures.
+  wp_loadField. wp_load. wp_apply (wp_WriteInt with "[$]"). iIntros (?) "Hsl". wp_store.
+  wp_loadField. wp_load. wp_apply (wp_WriteInt with "[$]"). iIntros (?) "Hsl". wp_store.
+  wp_loadField. wp_load. wp_apply (wp_WriteInt with "[$]"). iIntros (?) "Hsl". wp_store.
+  wp_loadField. wp_apply wp_boolToU64. wp_load.
+  wp_apply (wp_WriteInt with "[$]"). iIntros (?) "Hsl". wp_store.
+  iMod (readonly_load with "Hstate_sl") as (?) "Hstate_sl2".
+  wp_loadField. wp_load. wp_apply (wp_WriteBytes with "[$Hsl $Hstate_sl2]").
+  iIntros (?) "[Hsl _]". wp_store. wp_load.
+  iApply "HΦ".
+  iFrame. iExists _; by iFrame "∗#".
+Qed.
+
+Lemma wp_decode sl st :
+  {{{
+        own_slice_small sl byteT 1 (encode st)
+  }}}
+    decodePaxosState (slice_val sl)
+  {{{
+        s, RET #s; own_vol s st
+  }}}
+.
+Proof.
+  iIntros (?) "Hsl HΦ".
+  wp_lam. wp_apply wp_ref_to; first done.
+  iIntros (?) "He". wp_pures. wp_apply wp_ref_of_zero; first done.
+  iIntros (?) "HleaderInt". wp_pures. wp_apply (wp_allocStruct); first by val_ty.
+  iIntros (?) "Hs". iDestruct (struct_fields_split with "Hs") as "HH". iNamed "HH".
+  wp_pures. wp_load. wp_apply (wp_ReadInt with "[$]"). iIntros (?) "?".
+  wp_pures. wp_storeField. wp_store.
+  wp_load. wp_apply (wp_ReadInt with "[$]"). iIntros (?) "?".
+  wp_pures. wp_storeField. wp_store.
+  wp_load. wp_apply (wp_ReadInt with "[$]"). iIntros (?) "?".
+  wp_pures. wp_storeField. wp_store.
+  wp_load. wp_apply (wp_ReadInt with "[$]"). iIntros (?) "Hsl".
+  iMod (readonly_alloc_1 with "Hsl") as "#Hsl".
+  wp_pures. wp_store. wp_storeField. wp_load. wp_pures. wp_storeField.
+  iApply "HΦ".
+  iModIntro. repeat iExists _; iFrame "∗#".
+  iApply to_named. iExactEq "isLeader".
+  repeat f_equal. destruct st, isLeader; simpl.
+  { by rewrite bool_decide_eq_true. }
+  { by rewrite bool_decide_eq_false. }
+Qed.
+
+End paxosState.
+End paxosState.
